code/bignum/Hacl.Bignum.Exponentiation.fsti
@@ -11,6 +11,7 @@ open Hacl.Bignum.Definitions
 
 module S = Hacl.Spec.Bignum.Exponentiation
 module BN = Hacl.Bignum
+module BB = Hacl.Bignum.Base
 
 #reset-options "--z3rlimit 50 --fuel 0 --ifuel 0"
 
@@ -21,7 +22,7 @@ let check_mod_exp_st (nLen:BN.meta_len) =
   -> a:lbignum nLen
   -> bBits:size_t{0 < v bBits /\ 64 * v (blocks bBits 64ul) <= max_size_t}
   -> b:lbignum (blocks bBits 64ul) ->
-  Stack bool
+  Stack uint64
   (requires fun h ->
     live h n /\ live h a /\ live h b)
   (ensures  fun h0 r h1 -> modifies0 h0 h1 /\
@@ -85,7 +86,7 @@ let bn_mod_exp_st (nLen:BN.meta_len) =
     live h n /\ live h a /\ live h b /\ live h res /\
     disjoint res a /\ disjoint res b /\ disjoint res n /\ disjoint n a)
   (ensures  fun h0 r h1 -> modifies (loc res) h0 h1 /\
-    r == S.check_mod_exp (as_seq h0 n) (as_seq h0 a) (v bBits) (as_seq h0 b) /\
+    r == BB.unsafe_bool_of_u64 (S.check_mod_exp (as_seq h0 n) (as_seq h0 a) (v bBits) (as_seq h0 b)) /\
     r ==> S.bn_mod_exp_post #(v nLen) (as_seq h0 n) (as_seq h0 a) (v bBits) (as_seq h0 b) (as_seq h1 res))
 
 
